GraD/src/dqtt_ott.v
@@ -1,48 +1,56 @@
-Require Import Metalib.Metatheory.
-Require Export Metalib.LibLNgen.
- Require Export Qtt.usage_sig.
+Require Import Metalib.Metatheory. Require Export Metalib.LibLNgen. Require Export Qtt.usage_sig. 
 (** syntax *)
 Definition tmvar : Set := var. (*r variables *)
+Definition qvar : Set := var.
+Definition u : Set := usage.
 Definition index : Set := nat. (*r indices *)
 
-Definition usage : Set := usage.
+Inductive q : Set :=  (*r quantity, or usage expression *)
+ | q_Var_b (_:nat)
+ | q_Var_f (m:qvar)
+ | q_Const (u5:u)
+ | q_Plus (q1:q) (q2:q)
+ | q_Mul (q1:q) (q2:q).
 
 Inductive tm : Set :=  (*r terms and types *)
  | a_TyUnit : tm
  | a_TmUnit : tm
  | a_letunitB (a:tm) (b:tm) (B:tm)
- | a_Pi (q:usage) (A:tm) (B:tm)
- | a_Lam (q:usage) (A:tm) (a:tm)
+ | a_Pi (q5:q) (A:tm) (B:tm)
+ | a_Lam (q5:q) (A:tm) (a:tm)
  | a_App (a:tm) (b:tm)
- | a_Box (q:usage) (A:tm)
+ | a_Box (q5:q) (A:tm)
  | a_LetBoxB (a:tm) (b:tm) (B:tm)
  | a_Type : tm
  | a_Var_b (_:nat)
  | a_Var_f (x:tmvar)
- | a_box (q:usage) (a:tm)
+ | a_box (q5:q) (a:tm)
  | a_Let (a:tm) (b:tm)
  | a_Sum (A1:tm) (A2:tm)
  | a_Inj1 (a:tm)
  | a_Inj2 (a:tm)
- | a_Case (q:usage) (a:tm) (b1:tm) (b2:tm) (B:tm)
- | a_Sigma (q:usage) (A:tm) (B:tm)
+ | a_Case (q5:q) (a:tm) (b1:tm) (b2:tm) (B:tm)
+ | a_Sigma (q5:q) (A:tm) (B:tm)
  | a_Tensor (a:tm) (b:tm)
- | a_Spread (a:tm) (b:tm) (B:tm).
+ | a_Spread (a:tm) (b:tm) (B:tm)
+ | a_AllU (A:tm)
+ | a_LamU (a:tm)
+ | a_AppU (a:tm) (q5:q).
 
 Inductive sort : Set :=  (*r binding classifier *)
  | Tm (A:tm).
 
+Definition context : Set := list ( atom * (q * sort ) ).
+
 Definition D : Set := list ( atom * sort ).
 
-Definition context : Set := list ( atom * (usage * sort ) ).
-
-Definition heap : Set := list ( atom * ( usage * (context * tm * tm )) ).
+Definition heap : Set := list ( atom * ( q * (context * tm * tm )) ).
 
 Definition supp : Type := atoms.
 
-Definition n : Set := nat.
+Definition qlist : Set := list q.
 
-Definition qlist : Set := list usage.
+Definition n : Set := nat.
 
 (* EXPERIMENTAL *)
 (** auxiliary functions on the new list types *)
@@ -50,15 +58,29 @@ Definition qlist : Set := list usage.
 (** subrules *)
 (** arities *)
 (** opening up abstractions *)
+Fixpoint open_q_wrt_q_rec (k:nat) (r5:q) (r_6:q) {struct r_6}: q :=
+  match r_6 with
+  | (q_Var_b nat) => 
+      match lt_eq_lt_dec nat k with
+        | inleft (left _) => q_Var_b nat
+        | inleft (right _) => r5
+        | inright _ => q_Var_b (nat - 1)
+      end
+  | (q_Var_f m) => q_Var_f m
+  | (q_Const u5) => q_Const u5
+  | (q_Plus q1 q2) => q_Plus (open_q_wrt_q_rec k r5 q1) (open_q_wrt_q_rec k r5 q2)
+  | (q_Mul q1 q2) => q_Mul (open_q_wrt_q_rec k r5 q1) (open_q_wrt_q_rec k r5 q2)
+end.
+
 Fixpoint open_tm_wrt_tm_rec (k:nat) (a5:tm) (a_6:tm) {struct a_6}: tm :=
   match a_6 with
   | a_TyUnit => a_TyUnit 
   | a_TmUnit => a_TmUnit 
   | (a_letunitB a b B) => a_letunitB (open_tm_wrt_tm_rec k a5 a) (open_tm_wrt_tm_rec k a5 b) (open_tm_wrt_tm_rec k a5 B)
-  | (a_Pi q A B) => a_Pi q (open_tm_wrt_tm_rec k a5 A) (open_tm_wrt_tm_rec (S k) a5 B)
-  | (a_Lam q A a) => a_Lam q (open_tm_wrt_tm_rec k a5 A) (open_tm_wrt_tm_rec (S k) a5 a)
+  | (a_Pi q5 A B) => a_Pi q5 (open_tm_wrt_tm_rec k a5 A) (open_tm_wrt_tm_rec (S k) a5 B)
+  | (a_Lam q5 A a) => a_Lam q5 (open_tm_wrt_tm_rec k a5 A) (open_tm_wrt_tm_rec (S k) a5 a)
   | (a_App a b) => a_App (open_tm_wrt_tm_rec k a5 a) (open_tm_wrt_tm_rec k a5 b)
-  | (a_Box q A) => a_Box q (open_tm_wrt_tm_rec k a5 A)
+  | (a_Box q5 A) => a_Box q5 (open_tm_wrt_tm_rec k a5 A)
   | (a_LetBoxB a b B) => a_LetBoxB (open_tm_wrt_tm_rec k a5 a) (open_tm_wrt_tm_rec (S k) a5 b) (open_tm_wrt_tm_rec k a5 B)
   | a_Type => a_Type 
   | (a_Var_b nat) => 
@@ -68,15 +90,45 @@ Fixpoint open_tm_wrt_tm_rec (k:nat) (a5:tm) (a_6:tm) {struct a_6}: tm :=
         | inright _ => a_Var_b (nat - 1)
       end
   | (a_Var_f x) => a_Var_f x
-  | (a_box q a) => a_box q (open_tm_wrt_tm_rec k a5 a)
+  | (a_box q5 a) => a_box q5 (open_tm_wrt_tm_rec k a5 a)
   | (a_Let a b) => a_Let (open_tm_wrt_tm_rec k a5 a) (open_tm_wrt_tm_rec (S k) a5 b)
   | (a_Sum A1 A2) => a_Sum (open_tm_wrt_tm_rec k a5 A1) (open_tm_wrt_tm_rec k a5 A2)
   | (a_Inj1 a) => a_Inj1 (open_tm_wrt_tm_rec k a5 a)
   | (a_Inj2 a) => a_Inj2 (open_tm_wrt_tm_rec k a5 a)
-  | (a_Case q a b1 b2 B) => a_Case q (open_tm_wrt_tm_rec k a5 a) (open_tm_wrt_tm_rec k a5 b1) (open_tm_wrt_tm_rec k a5 b2) (open_tm_wrt_tm_rec k a5 B)
-  | (a_Sigma q A B) => a_Sigma q (open_tm_wrt_tm_rec k a5 A) (open_tm_wrt_tm_rec (S k) a5 B)
+  | (a_Case q5 a b1 b2 B) => a_Case q5 (open_tm_wrt_tm_rec k a5 a) (open_tm_wrt_tm_rec k a5 b1) (open_tm_wrt_tm_rec k a5 b2) (open_tm_wrt_tm_rec k a5 B)
+  | (a_Sigma q5 A B) => a_Sigma q5 (open_tm_wrt_tm_rec k a5 A) (open_tm_wrt_tm_rec (S k) a5 B)
   | (a_Tensor a b) => a_Tensor (open_tm_wrt_tm_rec k a5 a) (open_tm_wrt_tm_rec k a5 b)
   | (a_Spread a b B) => a_Spread (open_tm_wrt_tm_rec k a5 a) (open_tm_wrt_tm_rec (S k) a5 b) (open_tm_wrt_tm_rec k a5 B)
+  | (a_AllU A) => a_AllU (open_tm_wrt_tm_rec k a5 A)
+  | (a_LamU a) => a_LamU (open_tm_wrt_tm_rec k a5 a)
+  | (a_AppU a q5) => a_AppU (open_tm_wrt_tm_rec k a5 a) q5
+end.
+
+Fixpoint open_tm_wrt_q_rec (k:nat) (r5:q) (a5:tm) {struct a5}: tm :=
+  match a5 with
+  | a_TyUnit => a_TyUnit 
+  | a_TmUnit => a_TmUnit 
+  | (a_letunitB a b B) => a_letunitB (open_tm_wrt_q_rec k r5 a) (open_tm_wrt_q_rec k r5 b) (open_tm_wrt_q_rec k r5 B)
+  | (a_Pi q5 A B) => a_Pi (open_q_wrt_q_rec k r5 q5) (open_tm_wrt_q_rec k r5 A) (open_tm_wrt_q_rec k r5 B)
+  | (a_Lam q5 A a) => a_Lam (open_q_wrt_q_rec k r5 q5) (open_tm_wrt_q_rec k r5 A) (open_tm_wrt_q_rec k r5 a)
+  | (a_App a b) => a_App (open_tm_wrt_q_rec k r5 a) (open_tm_wrt_q_rec k r5 b)
+  | (a_Box q5 A) => a_Box (open_q_wrt_q_rec k r5 q5) (open_tm_wrt_q_rec k r5 A)
+  | (a_LetBoxB a b B) => a_LetBoxB (open_tm_wrt_q_rec k r5 a) (open_tm_wrt_q_rec k r5 b) (open_tm_wrt_q_rec k r5 B)
+  | a_Type => a_Type 
+  | (a_Var_b nat) => a_Var_b nat
+  | (a_Var_f x) => a_Var_f x
+  | (a_box q5 a) => a_box (open_q_wrt_q_rec k r5 q5) (open_tm_wrt_q_rec k r5 a)
+  | (a_Let a b) => a_Let (open_tm_wrt_q_rec k r5 a) (open_tm_wrt_q_rec k r5 b)
+  | (a_Sum A1 A2) => a_Sum (open_tm_wrt_q_rec k r5 A1) (open_tm_wrt_q_rec k r5 A2)
+  | (a_Inj1 a) => a_Inj1 (open_tm_wrt_q_rec k r5 a)
+  | (a_Inj2 a) => a_Inj2 (open_tm_wrt_q_rec k r5 a)
+  | (a_Case q5 a b1 b2 B) => a_Case (open_q_wrt_q_rec k r5 q5) (open_tm_wrt_q_rec k r5 a) (open_tm_wrt_q_rec k r5 b1) (open_tm_wrt_q_rec k r5 b2) (open_tm_wrt_q_rec k r5 B)
+  | (a_Sigma q5 A B) => a_Sigma (open_q_wrt_q_rec k r5 q5) (open_tm_wrt_q_rec k r5 A) (open_tm_wrt_q_rec k r5 B)
+  | (a_Tensor a b) => a_Tensor (open_tm_wrt_q_rec k r5 a) (open_tm_wrt_q_rec k r5 b)
+  | (a_Spread a b B) => a_Spread (open_tm_wrt_q_rec k r5 a) (open_tm_wrt_q_rec k r5 b) (open_tm_wrt_q_rec k r5 B)
+  | (a_AllU A) => a_AllU (open_tm_wrt_q_rec (S k) r5 A)
+  | (a_LamU a) => a_LamU (open_tm_wrt_q_rec (S k) r5 a)
+  | (a_AppU a q5) => a_AppU (open_tm_wrt_q_rec k r5 a) (open_q_wrt_q_rec k r5 q5)
 end.
 
 Definition open_sort_wrt_tm_rec (k:nat) (a5:tm) (sort5:sort) : sort :=
@@ -84,12 +136,38 @@ Definition open_sort_wrt_tm_rec (k:nat) (a5:tm) (sort5:sort) : sort :=
   | (Tm A) => Tm (open_tm_wrt_tm_rec k a5 A)
 end.
 
+Definition open_sort_wrt_q_rec (k:nat) (r5:q) (sort5:sort) : sort :=
+  match sort5 with
+  | (Tm A) => Tm (open_tm_wrt_q_rec k r5 A)
+end.
+
 Definition open_sort_wrt_tm a5 sort5 := open_sort_wrt_tm_rec 0 sort5 a5.
+
+Definition open_tm_wrt_q r5 a5 := open_tm_wrt_q_rec 0 a5 r5.
+
+Definition open_sort_wrt_q r5 sort5 := open_sort_wrt_q_rec 0 sort5 r5.
 
 Definition open_tm_wrt_tm a5 a_6 := open_tm_wrt_tm_rec 0 a_6 a5.
 
+Definition open_q_wrt_q r5 r_6 := open_q_wrt_q_rec 0 r_6 r5.
+
 (** terms are locally-closed pre-terms *)
 (** definitions *)
+
+(* defns LC_q *)
+Inductive lc_q : q -> Prop :=    (* defn lc_q *)
+ | lc_q_Var_f : forall (m:qvar),
+     (lc_q (q_Var_f m))
+ | lc_q_Const : forall (u5:u),
+     (lc_q (q_Const u5))
+ | lc_q_Plus : forall (q1 q2:q),
+     (lc_q q1) ->
+     (lc_q q2) ->
+     (lc_q (q_Plus q1 q2))
+ | lc_q_Mul : forall (q1 q2:q),
+     (lc_q q1) ->
+     (lc_q q2) ->
+     (lc_q (q_Mul q1 q2)).
 
 (* defns LC_tm *)
 Inductive lc_tm : tm -> Prop :=    (* defn lc_tm *)
@@ -102,21 +180,24 @@ Inductive lc_tm : tm -> Prop :=    (* defn lc_tm *)
      (lc_tm b) ->
      (lc_tm B) ->
      (lc_tm (a_letunitB a b B))
- | lc_a_Pi : forall (q:usage) (A B:tm),
+ | lc_a_Pi : forall (q5:q) (A B:tm),
+     (lc_q q5) ->
      (lc_tm A) ->
       ( forall x , lc_tm  ( open_tm_wrt_tm B (a_Var_f x) )  )  ->
-     (lc_tm (a_Pi q A B))
- | lc_a_Lam : forall (q:usage) (A a:tm),
+     (lc_tm (a_Pi q5 A B))
+ | lc_a_Lam : forall (q5:q) (A a:tm),
+     (lc_q q5) ->
      (lc_tm A) ->
       ( forall x , lc_tm  ( open_tm_wrt_tm a (a_Var_f x) )  )  ->
-     (lc_tm (a_Lam q A a))
+     (lc_tm (a_Lam q5 A a))
  | lc_a_App : forall (a b:tm),
      (lc_tm a) ->
      (lc_tm b) ->
      (lc_tm (a_App a b))
- | lc_a_Box : forall (q:usage) (A:tm),
+ | lc_a_Box : forall (q5:q) (A:tm),
+     (lc_q q5) ->
      (lc_tm A) ->
-     (lc_tm (a_Box q A))
+     (lc_tm (a_Box q5 A))
  | lc_a_LetBoxB : forall (a b B:tm),
      (lc_tm a) ->
       ( forall x , lc_tm  ( open_tm_wrt_tm b (a_Var_f x) )  )  ->
@@ -126,9 +207,10 @@ Inductive lc_tm : tm -> Prop :=    (* defn lc_tm *)
      (lc_tm a_Type)
  | lc_a_Var_f : forall (x:tmvar),
      (lc_tm (a_Var_f x))
- | lc_a_box : forall (q:usage) (a:tm),
+ | lc_a_box : forall (q5:q) (a:tm),
+     (lc_q q5) ->
      (lc_tm a) ->
-     (lc_tm (a_box q a))
+     (lc_tm (a_box q5 a))
  | lc_a_Let : forall (a b:tm),
      (lc_tm a) ->
       ( forall x , lc_tm  ( open_tm_wrt_tm b (a_Var_f x) )  )  ->
@@ -143,16 +225,18 @@ Inductive lc_tm : tm -> Prop :=    (* defn lc_tm *)
  | lc_a_Inj2 : forall (a:tm),
      (lc_tm a) ->
      (lc_tm (a_Inj2 a))
- | lc_a_Case : forall (q:usage) (a b1 b2 B:tm),
+ | lc_a_Case : forall (q5:q) (a b1 b2 B:tm),
+     (lc_q q5) ->
      (lc_tm a) ->
      (lc_tm b1) ->
      (lc_tm b2) ->
      (lc_tm B) ->
-     (lc_tm (a_Case q a b1 b2 B))
- | lc_a_Sigma : forall (q:usage) (A B:tm),
+     (lc_tm (a_Case q5 a b1 b2 B))
+ | lc_a_Sigma : forall (q5:q) (A B:tm),
+     (lc_q q5) ->
      (lc_tm A) ->
       ( forall x , lc_tm  ( open_tm_wrt_tm B (a_Var_f x) )  )  ->
-     (lc_tm (a_Sigma q A B))
+     (lc_tm (a_Sigma q5 A B))
  | lc_a_Tensor : forall (a b:tm),
      (lc_tm a) ->
      (lc_tm b) ->
@@ -161,7 +245,17 @@ Inductive lc_tm : tm -> Prop :=    (* defn lc_tm *)
      (lc_tm a) ->
       ( forall x , lc_tm  ( open_tm_wrt_tm b (a_Var_f x) )  )  ->
      (lc_tm B) ->
-     (lc_tm (a_Spread a b B)).
+     (lc_tm (a_Spread a b B))
+ | lc_a_AllU : forall (A:tm),
+      ( forall m , lc_tm  ( open_tm_wrt_q A (q_Var_f m) )  )  ->
+     (lc_tm (a_AllU A))
+ | lc_a_LamU : forall (a:tm),
+      ( forall m , lc_tm  ( open_tm_wrt_q a (q_Var_f m) )  )  ->
+     (lc_tm (a_LamU a))
+ | lc_a_AppU : forall (a:tm) (q5:q),
+     (lc_tm a) ->
+     (lc_q q5) ->
+     (lc_tm (a_AppU a q5)).
 
 (* defns LC_sort *)
 Inductive lc_sort : sort -> Prop :=    (* defn lc_sort *)
@@ -169,28 +263,67 @@ Inductive lc_sort : sort -> Prop :=    (* defn lc_sort *)
      (lc_tm A) ->
      (lc_sort (Tm A)).
 (** free variables *)
+Fixpoint fv_q_q (r5:q) : vars :=
+  match r5 with
+  | (q_Var_b nat) => {}
+  | (q_Var_f m) => {{m}}
+  | (q_Const u5) => {}
+  | (q_Plus q1 q2) => (fv_q_q q1) \u (fv_q_q q2)
+  | (q_Mul q1 q2) => (fv_q_q q1) \u (fv_q_q q2)
+end.
+
 Fixpoint fv_tm_tm (a5:tm) : vars :=
   match a5 with
   | a_TyUnit => {}
   | a_TmUnit => {}
   | (a_letunitB a b B) => (fv_tm_tm a) \u (fv_tm_tm b) \u (fv_tm_tm B)
-  | (a_Pi q A B) => (fv_tm_tm A) \u (fv_tm_tm B)
-  | (a_Lam q A a) => (fv_tm_tm A) \u (fv_tm_tm a)
+  | (a_Pi q5 A B) => (fv_tm_tm A) \u (fv_tm_tm B)
+  | (a_Lam q5 A a) => (fv_tm_tm A) \u (fv_tm_tm a)
   | (a_App a b) => (fv_tm_tm a) \u (fv_tm_tm b)
-  | (a_Box q A) => (fv_tm_tm A)
+  | (a_Box q5 A) => (fv_tm_tm A)
   | (a_LetBoxB a b B) => (fv_tm_tm a) \u (fv_tm_tm b) \u (fv_tm_tm B)
   | a_Type => {}
   | (a_Var_b nat) => {}
   | (a_Var_f x) => {{x}}
-  | (a_box q a) => (fv_tm_tm a)
+  | (a_box q5 a) => (fv_tm_tm a)
   | (a_Let a b) => (fv_tm_tm a) \u (fv_tm_tm b)
   | (a_Sum A1 A2) => (fv_tm_tm A1) \u (fv_tm_tm A2)
   | (a_Inj1 a) => (fv_tm_tm a)
   | (a_Inj2 a) => (fv_tm_tm a)
-  | (a_Case q a b1 b2 B) => (fv_tm_tm a) \u (fv_tm_tm b1) \u (fv_tm_tm b2) \u (fv_tm_tm B)
-  | (a_Sigma q A B) => (fv_tm_tm A) \u (fv_tm_tm B)
+  | (a_Case q5 a b1 b2 B) => (fv_tm_tm a) \u (fv_tm_tm b1) \u (fv_tm_tm b2) \u (fv_tm_tm B)
+  | (a_Sigma q5 A B) => (fv_tm_tm A) \u (fv_tm_tm B)
   | (a_Tensor a b) => (fv_tm_tm a) \u (fv_tm_tm b)
   | (a_Spread a b B) => (fv_tm_tm a) \u (fv_tm_tm b) \u (fv_tm_tm B)
+  | (a_AllU A) => (fv_tm_tm A)
+  | (a_LamU a) => (fv_tm_tm a)
+  | (a_AppU a q5) => (fv_tm_tm a)
+end.
+
+Fixpoint fv_q_tm (a5:tm) : vars :=
+  match a5 with
+  | a_TyUnit => {}
+  | a_TmUnit => {}
+  | (a_letunitB a b B) => (fv_q_tm a) \u (fv_q_tm b) \u (fv_q_tm B)
+  | (a_Pi q5 A B) => (fv_q_q q5) \u (fv_q_tm A) \u (fv_q_tm B)
+  | (a_Lam q5 A a) => (fv_q_q q5) \u (fv_q_tm A) \u (fv_q_tm a)
+  | (a_App a b) => (fv_q_tm a) \u (fv_q_tm b)
+  | (a_Box q5 A) => (fv_q_q q5) \u (fv_q_tm A)
+  | (a_LetBoxB a b B) => (fv_q_tm a) \u (fv_q_tm b) \u (fv_q_tm B)
+  | a_Type => {}
+  | (a_Var_b nat) => {}
+  | (a_Var_f x) => {}
+  | (a_box q5 a) => (fv_q_q q5) \u (fv_q_tm a)
+  | (a_Let a b) => (fv_q_tm a) \u (fv_q_tm b)
+  | (a_Sum A1 A2) => (fv_q_tm A1) \u (fv_q_tm A2)
+  | (a_Inj1 a) => (fv_q_tm a)
+  | (a_Inj2 a) => (fv_q_tm a)
+  | (a_Case q5 a b1 b2 B) => (fv_q_q q5) \u (fv_q_tm a) \u (fv_q_tm b1) \u (fv_q_tm b2) \u (fv_q_tm B)
+  | (a_Sigma q5 A B) => (fv_q_q q5) \u (fv_q_tm A) \u (fv_q_tm B)
+  | (a_Tensor a b) => (fv_q_tm a) \u (fv_q_tm b)
+  | (a_Spread a b B) => (fv_q_tm a) \u (fv_q_tm b) \u (fv_q_tm B)
+  | (a_AllU A) => (fv_q_tm A)
+  | (a_LamU a) => (fv_q_tm a)
+  | (a_AppU a q5) => (fv_q_tm a) \u (fv_q_q q5)
 end.
 
 Definition fv_tm_sort (sort5:sort) : vars :=
@@ -198,34 +331,83 @@ Definition fv_tm_sort (sort5:sort) : vars :=
   | (Tm A) => (fv_tm_tm A)
 end.
 
+Definition fv_q_sort (sort5:sort) : vars :=
+  match sort5 with
+  | (Tm A) => (fv_q_tm A)
+end.
+
 (** substitutions *)
+Fixpoint subst_q_q (r5:q) (m5:qvar) (r_6:q) {struct r_6} : q :=
+  match r_6 with
+  | (q_Var_b nat) => q_Var_b nat
+  | (q_Var_f m) => (if eq_var m m5 then r5 else (q_Var_f m))
+  | (q_Const u5) => q_Const u5
+  | (q_Plus q1 q2) => q_Plus (subst_q_q r5 m5 q1) (subst_q_q r5 m5 q2)
+  | (q_Mul q1 q2) => q_Mul (subst_q_q r5 m5 q1) (subst_q_q r5 m5 q2)
+end.
+
 Fixpoint subst_tm_tm (a5:tm) (x5:tmvar) (a_6:tm) {struct a_6} : tm :=
   match a_6 with
   | a_TyUnit => a_TyUnit 
   | a_TmUnit => a_TmUnit 
   | (a_letunitB a b B) => a_letunitB (subst_tm_tm a5 x5 a) (subst_tm_tm a5 x5 b) (subst_tm_tm a5 x5 B)
-  | (a_Pi q A B) => a_Pi q (subst_tm_tm a5 x5 A) (subst_tm_tm a5 x5 B)
-  | (a_Lam q A a) => a_Lam q (subst_tm_tm a5 x5 A) (subst_tm_tm a5 x5 a)
+  | (a_Pi q5 A B) => a_Pi q5 (subst_tm_tm a5 x5 A) (subst_tm_tm a5 x5 B)
+  | (a_Lam q5 A a) => a_Lam q5 (subst_tm_tm a5 x5 A) (subst_tm_tm a5 x5 a)
   | (a_App a b) => a_App (subst_tm_tm a5 x5 a) (subst_tm_tm a5 x5 b)
-  | (a_Box q A) => a_Box q (subst_tm_tm a5 x5 A)
+  | (a_Box q5 A) => a_Box q5 (subst_tm_tm a5 x5 A)
   | (a_LetBoxB a b B) => a_LetBoxB (subst_tm_tm a5 x5 a) (subst_tm_tm a5 x5 b) (subst_tm_tm a5 x5 B)
   | a_Type => a_Type 
   | (a_Var_b nat) => a_Var_b nat
   | (a_Var_f x) => (if eq_var x x5 then a5 else (a_Var_f x))
-  | (a_box q a) => a_box q (subst_tm_tm a5 x5 a)
+  | (a_box q5 a) => a_box q5 (subst_tm_tm a5 x5 a)
   | (a_Let a b) => a_Let (subst_tm_tm a5 x5 a) (subst_tm_tm a5 x5 b)
   | (a_Sum A1 A2) => a_Sum (subst_tm_tm a5 x5 A1) (subst_tm_tm a5 x5 A2)
   | (a_Inj1 a) => a_Inj1 (subst_tm_tm a5 x5 a)
   | (a_Inj2 a) => a_Inj2 (subst_tm_tm a5 x5 a)
-  | (a_Case q a b1 b2 B) => a_Case q (subst_tm_tm a5 x5 a) (subst_tm_tm a5 x5 b1) (subst_tm_tm a5 x5 b2) (subst_tm_tm a5 x5 B)
-  | (a_Sigma q A B) => a_Sigma q (subst_tm_tm a5 x5 A) (subst_tm_tm a5 x5 B)
+  | (a_Case q5 a b1 b2 B) => a_Case q5 (subst_tm_tm a5 x5 a) (subst_tm_tm a5 x5 b1) (subst_tm_tm a5 x5 b2) (subst_tm_tm a5 x5 B)
+  | (a_Sigma q5 A B) => a_Sigma q5 (subst_tm_tm a5 x5 A) (subst_tm_tm a5 x5 B)
   | (a_Tensor a b) => a_Tensor (subst_tm_tm a5 x5 a) (subst_tm_tm a5 x5 b)
   | (a_Spread a b B) => a_Spread (subst_tm_tm a5 x5 a) (subst_tm_tm a5 x5 b) (subst_tm_tm a5 x5 B)
+  | (a_AllU A) => a_AllU (subst_tm_tm a5 x5 A)
+  | (a_LamU a) => a_LamU (subst_tm_tm a5 x5 a)
+  | (a_AppU a q5) => a_AppU (subst_tm_tm a5 x5 a) q5
+end.
+
+Fixpoint subst_q_tm (r5:q) (m5:qvar) (a5:tm) {struct a5} : tm :=
+  match a5 with
+  | a_TyUnit => a_TyUnit 
+  | a_TmUnit => a_TmUnit 
+  | (a_letunitB a b B) => a_letunitB (subst_q_tm r5 m5 a) (subst_q_tm r5 m5 b) (subst_q_tm r5 m5 B)
+  | (a_Pi q5 A B) => a_Pi (subst_q_q r5 m5 q5) (subst_q_tm r5 m5 A) (subst_q_tm r5 m5 B)
+  | (a_Lam q5 A a) => a_Lam (subst_q_q r5 m5 q5) (subst_q_tm r5 m5 A) (subst_q_tm r5 m5 a)
+  | (a_App a b) => a_App (subst_q_tm r5 m5 a) (subst_q_tm r5 m5 b)
+  | (a_Box q5 A) => a_Box (subst_q_q r5 m5 q5) (subst_q_tm r5 m5 A)
+  | (a_LetBoxB a b B) => a_LetBoxB (subst_q_tm r5 m5 a) (subst_q_tm r5 m5 b) (subst_q_tm r5 m5 B)
+  | a_Type => a_Type 
+  | (a_Var_b nat) => a_Var_b nat
+  | (a_Var_f x) => a_Var_f x
+  | (a_box q5 a) => a_box (subst_q_q r5 m5 q5) (subst_q_tm r5 m5 a)
+  | (a_Let a b) => a_Let (subst_q_tm r5 m5 a) (subst_q_tm r5 m5 b)
+  | (a_Sum A1 A2) => a_Sum (subst_q_tm r5 m5 A1) (subst_q_tm r5 m5 A2)
+  | (a_Inj1 a) => a_Inj1 (subst_q_tm r5 m5 a)
+  | (a_Inj2 a) => a_Inj2 (subst_q_tm r5 m5 a)
+  | (a_Case q5 a b1 b2 B) => a_Case (subst_q_q r5 m5 q5) (subst_q_tm r5 m5 a) (subst_q_tm r5 m5 b1) (subst_q_tm r5 m5 b2) (subst_q_tm r5 m5 B)
+  | (a_Sigma q5 A B) => a_Sigma (subst_q_q r5 m5 q5) (subst_q_tm r5 m5 A) (subst_q_tm r5 m5 B)
+  | (a_Tensor a b) => a_Tensor (subst_q_tm r5 m5 a) (subst_q_tm r5 m5 b)
+  | (a_Spread a b B) => a_Spread (subst_q_tm r5 m5 a) (subst_q_tm r5 m5 b) (subst_q_tm r5 m5 B)
+  | (a_AllU A) => a_AllU (subst_q_tm r5 m5 A)
+  | (a_LamU a) => a_LamU (subst_q_tm r5 m5 a)
+  | (a_AppU a q5) => a_AppU (subst_q_tm r5 m5 a) (subst_q_q r5 m5 q5)
 end.
 
 Definition subst_tm_sort (a5:tm) (x5:tmvar) (sort5:sort) : sort :=
   match sort5 with
   | (Tm A) => Tm (subst_tm_tm a5 x5 A)
+end.
+
+Definition subst_q_sort (r5:q) (m5:qvar) (sort5:sort) : sort :=
+  match sort5 with
+  | (Tm A) => Tm (subst_q_tm r5 m5 A)
 end.
 
 
@@ -261,9 +443,44 @@ Fixpoint close_tm_wrt_tm_rec (n1 : nat) (x1 : tmvar) (a1 : tm) {struct a1} : tm 
     | a_Sigma q1 A1 B1 => a_Sigma q1 (close_tm_wrt_tm_rec n1 x1 A1) (close_tm_wrt_tm_rec (S n1) x1 B1)
     | a_Tensor a2 b1 => a_Tensor (close_tm_wrt_tm_rec n1 x1 a2) (close_tm_wrt_tm_rec n1 x1 b1)
     | a_Spread a2 b1 B1 => a_Spread (close_tm_wrt_tm_rec n1 x1 a2) (close_tm_wrt_tm_rec (S n1) x1 b1) (close_tm_wrt_tm_rec n1 x1 B1)
+    | a_AllU A => a_AllU (close_tm_wrt_tm_rec (S n1) x1 A)
+    | a_LamU a => a_LamU (close_tm_wrt_tm_rec (S n1) x1 a)
+    | a_AppU a u => a_AppU (close_tm_wrt_tm_rec n1 x1 a) u
   end.
 
 Definition close_tm_wrt_tm x1 a1 := close_tm_wrt_tm_rec 0 x1 a1.
+
+Definition sort_mul {A} (q1: q) (s : q * A) : q * A :=
+  match s with 
+  | (q2 , A) => (q_Mul q1 q2, A)
+  end.
+
+Definition ctx_mul {A} (q1 : q) (G : list (var * (q * A))) := 
+  map (sort_mul q1) G.
+
+Fixpoint ctx_plus {A} (G1 G2 : list (var * (q * A))) : list (var * (q * A)) :=
+  match G1, G2 with 
+  | nil , nil => nil
+  | cons (x , (q1 , A)) G1' , cons (_, (q2, _)) G2' => cons (x, (q_Plus q1 q2, A)) (ctx_plus G1' G2')
+  | _ , _ => nil
+  end.
+
+
+Inductive ctx {A} : list (atom * A) -> list (atom * (q * A)) -> Prop :=  
+ | ctx_nil : 
+     ctx nil nil 
+ | ctx_cons : forall D (x:atom) G (q1:q) a,
+     ctx D G ->
+      ~ AtomSetImpl.In x (dom  D)  ->
+     ctx (x ~ a ++ D ) (x ~ (q1,a) ++ G).
+
+Arguments sort_mul {_}.
+Arguments ctx_mul {_}.
+Arguments ctx_plus {_}.
+Arguments ctx {_}.
+
+Hint Constructors ctx : core.
+
 
 
 (** definitions *)
@@ -274,11 +491,12 @@ Inductive Step : tm -> tm -> Prop :=    (* defn Step *)
      lc_tm b ->
      Step a a' ->
      Step (a_App a b) (a_App a' b)
- | S_Beta : forall (q:usage) (A a b:tm),
+ | S_Beta : forall (q5:q) (A a b:tm),
+     lc_q q5 ->
      lc_tm A ->
-     lc_tm (a_Lam q A a) ->
+     lc_tm (a_Lam q5 A a) ->
      lc_tm b ->
-     Step (a_App  ( (a_Lam q A a) )  b)  (open_tm_wrt_tm  a   b ) 
+     Step (a_App  ( (a_Lam q5 A a) )  b)  (open_tm_wrt_tm  a   b ) 
  | S_UnitCong : forall (a b B a':tm),
      lc_tm b ->
      lc_tm B ->
@@ -293,29 +511,33 @@ Inductive Step : tm -> tm -> Prop :=    (* defn Step *)
      lc_tm B ->
      Step a a' ->
      Step (a_LetBoxB a b B) (a_LetBoxB a' b B)
- | S_BoxBeta : forall (q:usage) (a b B:tm),
-     lc_tm (a_LetBoxB (a_box q a) b B) ->
+ | S_BoxBeta : forall (q5:q) (a b B:tm),
+     lc_q q5 ->
+     lc_tm (a_LetBoxB (a_box q5 a) b B) ->
      lc_tm B ->
      lc_tm a ->
-     Step (a_LetBoxB (a_box q a) b B)  (open_tm_wrt_tm  b   a ) 
- | S_CaseCong : forall (q:usage) (a b1 b2 B a':tm),
+     Step (a_LetBoxB (a_box q5 a) b B)  (open_tm_wrt_tm  b   a ) 
+ | S_CaseCong : forall (q5:q) (a b1 b2 B a':tm),
+     lc_q q5 ->
      lc_tm b1 ->
      lc_tm b2 ->
      lc_tm B ->
      Step a a' ->
-     Step (a_Case q a b1 b2 B) (a_Case q a' b1 b2 B)
- | S_Case1Beta : forall (q:usage) (a b1 b2 B:tm),
+     Step (a_Case q5 a b1 b2 B) (a_Case q5 a' b1 b2 B)
+ | S_Case1Beta : forall (q5:q) (a b1 b2 B:tm),
+     lc_q q5 ->
      lc_tm b2 ->
      lc_tm B ->
      lc_tm b1 ->
      lc_tm a ->
-     Step (a_Case q  ( (a_Inj1 a) )  b1 b2 B) (a_App b1 a)
- | S_Case2Beta : forall (q:usage) (a b1 b2 B:tm),
+     Step (a_Case q5  ( (a_Inj1 a) )  b1 b2 B) (a_App b1 a)
+ | S_Case2Beta : forall (q5:q) (a b1 b2 B:tm),
+     lc_q q5 ->
      lc_tm b1 ->
      lc_tm B ->
      lc_tm b2 ->
      lc_tm a ->
-     Step (a_Case q  ( (a_Inj2 a) )  b1 b2 B) (a_App b2 a)
+     Step (a_Case q5  ( (a_Inj2 a) )  b1 b2 B) (a_App b2 a)
  | S_SpreadCong : forall (a b B a':tm),
      lc_tm (a_Spread a b B) ->
      lc_tm B ->
@@ -328,35 +550,51 @@ Inductive Step : tm -> tm -> Prop :=    (* defn Step *)
      lc_tm a1 ->
      Step (a_Spread (a_Tensor a0 a1) b B) (a_App  (open_tm_wrt_tm  b   a0 )  a1).
 
+(* defns JSub *)
+Inductive q_sub : q -> q -> Prop :=    (* defn q_sub *)
+ | Const : forall (u1 u2:u),
+      ( u1  <=  u2 )  ->
+     q_sub (q_Const u1) (q_Const u2)
+with ctx_sub : D -> context -> context -> Prop :=    (* defn ctx_sub *)
+ | CS_Empty : 
+     ctx_sub  nil   nil   nil 
+ | CS_ConsTm : forall (D5:D) (x:tmvar) (A:tm) (G1:context) (q1:q) (G2:context) (q2:q),
+     lc_tm A ->
+     q_sub q1 q2 ->
+     ctx_sub D5 G1 G2 ->
+      ~ AtomSetImpl.In  x  (dom  D5 )  ->
+     ctx_sub  (  ( x  ~ Tm A )  ++ D5 )   (  ( x ~( q1 ,Tm  A ))  ++ G1 )   (  ( x ~( q2 ,Tm  A ))  ++ G2 ) .
+
 (* defns JTyping *)
 Inductive Typing : D -> context -> tm -> tm -> Prop :=    (* defn Typing *)
  | T_sub : forall (D5:D) (G2:context) (a A:tm) (G1:context),
      Typing D5 G1 a A ->
-      ctx_sub  D5   G1   G2  ->
+     ctx_sub D5 G1 G2 ->
      Typing D5 G2 a A
  | T_type : 
      Typing  nil   nil  a_Type a_Type
  | T_var : forall (D5:D) (x:tmvar) (A:tm) (G:context),
       ~ AtomSetImpl.In  x  (dom  D5 )  ->
      Typing D5 G A a_Type ->
-     Typing  (  ( x  ~ Tm A )  ++ D5 )   (  ( x ~(  1  ,Tm  A ))  ++   (ctx_mul   0    G )   )  (a_Var_f x) A
+     Typing  (  ( x  ~ Tm A )  ++ D5 )   (  ( x ~(  (q_Const 1)  ,Tm  A ))  ++   (ctx_mul   (q_Const 0)    G )   )  (a_Var_f x) A
  | T_weak : forall (D5:D) (x:tmvar) (A:tm) (G1:context) (a B:tm) (G2:context),
       ~ AtomSetImpl.In  x  (dom  D5 )  ->
      Typing D5 G1 a B ->
      Typing D5 G2 A a_Type ->
-     Typing  (  ( x  ~ Tm A )  ++ D5 )   (  ( x ~(  0  ,Tm  A ))  ++ G1 )  a B
- | T_pi : forall (L:vars) (D5:D) (G1 G2:context) (q:usage) (A B:tm) (r:usage),
+     Typing  (  ( x  ~ Tm A )  ++ D5 )   (  ( x ~(  (q_Const 0)  ,Tm  A ))  ++ G1 )  a B
+ | T_pi : forall (L:vars) (D5:D) (G1 G2:context) (q5:q) (A B:tm) (r:q),
+     lc_q q5 ->
      Typing D5 G1 A a_Type ->
       ( forall x , x \notin  L  -> Typing  (  ( x  ~ Tm A )  ++ D5 )   (  ( x ~( r ,Tm  A ))  ++ G2 )   ( open_tm_wrt_tm B (a_Var_f x) )  a_Type )  ->
-     Typing D5  (ctx_plus  G1   G2 )  (a_Pi q A B) a_Type
- | T_lam : forall (L:vars) (D5:D) (G1:context) (q:usage) (A a B:tm) (G2:context),
-      ( forall x , x \notin  L  -> Typing  (  ( x  ~ Tm A )  ++ D5 )   (  ( x ~( q ,Tm  A ))  ++ G1 )   ( open_tm_wrt_tm a (a_Var_f x) )   ( open_tm_wrt_tm B (a_Var_f x) )  )  ->
+     Typing D5  (ctx_plus  G1   G2 )  (a_Pi q5 A B) a_Type
+ | T_lam : forall (L:vars) (D5:D) (G1:context) (q5:q) (A a B:tm) (G2:context),
+      ( forall x , x \notin  L  -> Typing  (  ( x  ~ Tm A )  ++ D5 )   (  ( x ~( q5 ,Tm  A ))  ++ G1 )   ( open_tm_wrt_tm a (a_Var_f x) )   ( open_tm_wrt_tm B (a_Var_f x) )  )  ->
      Typing D5 G2 A a_Type ->
-     Typing D5 G1 (a_Lam q A a) (a_Pi q A B)
- | T_app : forall (D5:D) (G1:context) (q:usage) (G2:context) (a b B A:tm),
-     Typing D5 G1 a (a_Pi q A B) ->
+     Typing D5 G1 (a_Lam q5 A a) (a_Pi q5 A B)
+ | T_app : forall (D5:D) (G1:context) (q5:q) (G2:context) (a b B A:tm),
+     Typing D5 G1 a (a_Pi q5 A B) ->
      Typing D5 G2 b A ->
-     Typing D5  (ctx_plus  G1     (ctx_mul  q   G2 )   )  (a_App a b)  (open_tm_wrt_tm  B   b ) 
+     Typing D5  (ctx_plus  G1     (ctx_mul  q5   G2 )   )  (a_App a b)  (open_tm_wrt_tm  B   b ) 
  | T_conv : forall (D5:D) (G1:context) (a B A:tm) (G2:context),
      Typing D5 G1 a A ->
      Typing D5 G2 B a_Type ->
@@ -366,23 +604,25 @@ Inductive Typing : D -> context -> tm -> tm -> Prop :=    (* defn Typing *)
      Typing  nil   nil  a_TmUnit a_TyUnit
  | T_Unit : 
      Typing  nil   nil  a_TyUnit a_Type
- | T_UnitE : forall (L:vars) (D5:D) (G1 G2:context) (a b:tm) (r:usage) (B B1:tm) (G3:context),
+ | T_UnitE : forall (L:vars) (D5:D) (G1 G2:context) (a b:tm) (r:q) (B B1:tm) (G3:context),
      Typing D5 G1 a a_TyUnit ->
       B1 =  (open_tm_wrt_tm  B   a_TmUnit )   ->
      Typing D5 G2 b B1 ->
       ( forall y , y \notin  L  -> Typing  (  ( y  ~ Tm a_TyUnit )  ++ D5 )   (  ( y ~( r ,Tm  a_TyUnit ))  ++ G3 )   ( open_tm_wrt_tm B (a_Var_f y) )  a_Type )  ->
      Typing D5  (ctx_plus  G1   G2 )  (a_letunitB a b  ( (a_Lam r a_TyUnit B) ) )  (open_tm_wrt_tm  B   a ) 
- | T_Box : forall (D5:D) (G:context) (q:usage) (A:tm),
+ | T_Box : forall (D5:D) (G:context) (q5:q) (A:tm),
+     lc_q q5 ->
      Typing D5 G A a_Type ->
-     Typing D5 G (a_Box q A) a_Type
- | T_box : forall (D5:D) (q:usage) (G:context) (a A:tm),
+     Typing D5 G (a_Box q5 A) a_Type
+ | T_box : forall (D5:D) (q5:q) (G:context) (a A:tm),
+     lc_q q5 ->
      Typing D5 G a A ->
-     Typing D5  (ctx_mul  q   G )  (a_box q a) (a_Box q A)
- | T_letbox : forall (L:vars) (D5:D) (G1 G2:context) (a b:tm) (r q:usage) (A B:tm) (G3:context),
-     Typing D5 G1 a (a_Box q A) ->
-      ( forall x , x \notin  L  -> Typing  (  ( x  ~ Tm A )  ++ D5 )   (  ( x ~( q ,Tm  A ))  ++ G2 )   ( open_tm_wrt_tm b (a_Var_f x) )   (open_tm_wrt_tm  B   (a_box q (a_Var_f x)) )  )  ->
-      ( forall y , y \notin  L  -> Typing  (  ( y  ~ Tm (a_Box q A) )  ++ D5 )   (  ( y ~( r ,Tm  (a_Box q A) ))  ++ G3 )   ( open_tm_wrt_tm B (a_Var_f y) )  a_Type )  ->
-     Typing D5  (ctx_plus  G1   G2 )  (a_LetBoxB a b  ( (a_Lam r (a_Box q A) B) ) )  (open_tm_wrt_tm  B   a ) 
+     Typing D5  (ctx_mul  q5   G )  (a_box q5 a) (a_Box q5 A)
+ | T_letbox : forall (L:vars) (D5:D) (G1 G2:context) (a b:tm) (r q5:q) (A B:tm) (G3:context),
+     Typing D5 G1 a (a_Box q5 A) ->
+      ( forall x , x \notin  L  -> Typing  (  ( x  ~ Tm A )  ++ D5 )   (  ( x ~( q5 ,Tm  A ))  ++ G2 )   ( open_tm_wrt_tm b (a_Var_f x) )   (open_tm_wrt_tm  B   (a_box q5 (a_Var_f x)) )  )  ->
+      ( forall y , y \notin  L  -> Typing  (  ( y  ~ Tm (a_Box q5 A) )  ++ D5 )   (  ( y ~( r ,Tm  (a_Box q5 A) ))  ++ G3 )   ( open_tm_wrt_tm B (a_Var_f y) )  a_Type )  ->
+     Typing D5  (ctx_plus  G1   G2 )  (a_LetBoxB a b  ( (a_Lam r (a_Box q5 A) B) ) )  (open_tm_wrt_tm  B   a ) 
  | T_sum : forall (D5:D) (G1 G2:context) (A1 A2:tm),
      Typing D5 G1 A1 a_Type ->
      Typing D5 G2 A2 a_Type ->
@@ -395,37 +635,29 @@ Inductive Typing : D -> context -> tm -> tm -> Prop :=    (* defn Typing *)
      Typing D5 G a A2 ->
      Typing D5 G1 A1 a_Type ->
      Typing D5 G (a_Inj2 a) (a_Sum A1 A2)
- | T_case : forall (L:vars) (D5:D) (q:usage) (G1 G2:context) (a b1 b2:tm) (r:usage) (A1 A2 B B1 B2:tm) (G3:context),
-      (  1   <=  q )  ->
+ | T_case : forall (L:vars) (D5:D) (q5:q) (G1 G2:context) (a b1 b2:tm) (r:q) (A1 A2 B B1 B2:tm) (G3:context),
+     q_sub  (q_Const 1)  q5 ->
      Typing D5 G1 a (a_Sum A1 A2) ->
       ( forall x , x \notin  L  ->   ( open_tm_wrt_tm B1 (a_Var_f x) )  =   (open_tm_wrt_tm  B   (a_Inj1 (a_Var_f x)) )    )  ->
       ( forall x , x \notin  L  ->   ( open_tm_wrt_tm B2 (a_Var_f x) )  =   (open_tm_wrt_tm  B   (a_Inj2 (a_Var_f x)) )    )  ->
-     Typing D5 G2 b1 (a_Pi q A1 B1) ->
-     Typing D5 G2 b2 (a_Pi q A2 B2) ->
+     Typing D5 G2 b1 (a_Pi q5 A1 B1) ->
+     Typing D5 G2 b2 (a_Pi q5 A2 B2) ->
       ( forall y , y \notin  L  -> Typing  (  ( y  ~ Tm (a_Sum A1 A2) )  ++ D5 )   (  ( y ~( r ,Tm  (a_Sum A1 A2) ))  ++ G3 )   ( open_tm_wrt_tm B (a_Var_f y) )  a_Type )  ->
-     Typing D5  (ctx_plus    (ctx_mul  q   G1 )     G2 )  (a_Case q a b1 b2  ( (a_Lam r (a_Sum A1 A2) B) ) )  (open_tm_wrt_tm  B   a ) 
- | T_Sigma : forall (L:vars) (D5:D) (G1 G2:context) (q:usage) (A B:tm) (r:usage),
+     Typing D5  (ctx_plus    (ctx_mul  q5   G1 )     G2 )  (a_Case q5 a b1 b2  ( (a_Lam r (a_Sum A1 A2) B) ) )  (open_tm_wrt_tm  B   a ) 
+ | T_Sigma : forall (L:vars) (D5:D) (G1 G2:context) (q5:q) (A B:tm) (r:q),
+     lc_q q5 ->
      Typing D5 G1 A a_Type ->
       ( forall x , x \notin  L  -> Typing  (  ( x  ~ Tm A )  ++ D5 )   (  ( x ~( r ,Tm  A ))  ++ G2 )   ( open_tm_wrt_tm B (a_Var_f x) )  a_Type )  ->
-     Typing D5  (ctx_plus  G1   G2 )  (a_Sigma q A B) a_Type
- | T_Tensor : forall (L:vars) (D5:D) (q:usage) (G1 G2:context) (a b A B:tm) (G3:context) (r:usage),
+     Typing D5  (ctx_plus  G1   G2 )  (a_Sigma q5 A B) a_Type
+ | T_Tensor : forall (L:vars) (D5:D) (q5:q) (G1 G2:context) (a b A B:tm) (G3:context) (r:q),
+     lc_q q5 ->
      Typing D5 G1 a A ->
      Typing D5 G2 b  (open_tm_wrt_tm  B   a )  ->
       ( forall x , x \notin  L  -> Typing  (  ( x  ~ Tm A )  ++ D5 )   (  ( x ~( r ,Tm  A ))  ++ G3 )   ( open_tm_wrt_tm B (a_Var_f x) )  a_Type )  ->
-     Typing D5  (ctx_plus    (ctx_mul  q   G1 )     G2 )  (a_Tensor a b) (a_Sigma q A B)
- | T_Spread : forall (L:vars) (D5:D) (G1 G2:context) (a b:tm) (r:usage) (A B:tm) (q:usage) (A1 A2:tm) (G3:context),
-      A = (a_Sigma q A1 A2)  ->
-     Typing D5 G1 a A ->
-      ( forall x , x \notin L -> 
-        forall y, y \notin L \u {{x}} -> 
-           Typing  ((x ~ Tm A1) ++ D5) ((x ~( q ,Tm A1 )) ++ G2 ) (open_tm_wrt_tm b (a_Var_f x)) 
-               (a_Pi 1 (open_tm_wrt_tm A2 (a_Var_f x))
-                     (close_tm_wrt_tm y (open_tm_wrt_tm B (a_Tensor (a_Var_f x) (a_Var_f y))))))  ->
-      ( forall y , y \notin L -> Typing (y ~ Tm A ++ D5)  ((y ~(r , Tm A)) ++ G3)  (open_tm_wrt_tm B (a_Var_f y)) a_Type)  ->
-     Typing D5  (ctx_plus G1 G2)  (a_Spread a b  (a_Lam r A B))  (open_tm_wrt_tm B a) .
+     Typing D5  (ctx_plus    (ctx_mul  q5   G1 )     G2 )  (a_Tensor a b) (a_Sigma q5 A B).
 
 
 (** infrastructure *)
-Hint Constructors Step Typing lc_tm lc_sort : core.
+Hint Constructors Step q_sub ctx_sub Typing lc_q lc_tm lc_sort : core.
 
 
